everything ready before ystep

WeirdLogic/Example4.lean
@@ -17,12 +17,15 @@ open ContextFreeGrammar
 namespace WeirdLogic
 
 /- L -> (S1; S2)
-  S1 -> trm2; S1
+  S1 -> S3; S1
         | ε
   S2 -> trm 1
+  S3 -> trm 2 | trm 3
  -/
+
 def trm1 : trm := [lang| x := -x]
 def trm2 : trm := [lang| x := x + 1]
+def trm3 : trm := [lang| x := x * 2]
 def r1 : ContextFreeRule trm String :=
   {
     input := "L",
@@ -32,7 +35,7 @@ def r1 : ContextFreeRule trm String :=
 def r2 : ContextFreeRule trm String :=
   {
     input := "S1",
-    output := [Symbol.terminal trm2, Symbol.nonterminal "S1"],
+    output := [Symbol.nonterminal "S3", Symbol.nonterminal "S1"],
   }
 
 def r3 : ContextFreeRule trm String :=
@@ -47,64 +50,77 @@ def r4 : ContextFreeRule trm String :=
     output := [Symbol.terminal trm1],
   }
 
+def r5 : ContextFreeRule trm String :=
+  {
+    input := "S3",
+    output := [Symbol.terminal trm2],
+  }
+
+def r6 : ContextFreeRule trm String :=
+  {
+    input := "S3",
+    output := [Symbol.terminal trm3],
+  }
 
 def cfg1 : ContextFreeGrammar trm :=
   {
     NT := String,
     initial := "S1",
-    rules := Finset.mk {r1, r2, r3, r4} (by unfold r1 r2 r3 r4 trm1 trm2; simp)
+    rules := Finset.mk {r1, r2, r3, r4, r5, r6} (by unfold r1 r2 r3 r4 r5 r6 trm1 trm2 trm3; simp)
   }
 
 def l1 : Language trm := cfg1.language
 
--- lang_def prog_c1 :=
---   fun ⸨x: Val⸩ ⸨pa:Val⸩ =>
---     while pa > 0 {
---         x := x + 1;
---         pa := pa-1
---     };
---     x := -x
+-- def prog_c1 (pa pb : List ℤ) : val :=
+-- [trm|
+--   let i := 0
+--   let b := ⟨pa[i]⟩
+--   ...
+-- ]
+-- fun f : trm -> ℤ
+--
 
 lang_def prog_c1 :=
-  fun ⸨x: Val⸩ ⸨pa:Val⸩ =>
-    for i in [0:pa] {
-        x := x + 1
+  fun ⸨x: Val⸩ ⸨pa:Loc⸩ ⸨pb:Loc⸩ =>
+    let i := 0 in
+    let b := pb[i] in
+    while pb[i] {
+      let a := pa[i] in
+        if a > 0 then
+          x := x + 1
+        else
+          x := x*2;
+      i := i+1
     };
     x := -x
 
-abbrev default_payload : payload:= 0
+abbrev multi_payload := List ℤ
+
+abbrev default_payload : multi_payload:= [0]
 abbrev default_trm : trm := [lang|()]
 
-def pay_index : Set (trm × payload) :=
+def pay_index : Set (trm × multi_payload × multi_payload) :=
   {
-    ([lang|()],p) | p ∈ @Set.univ payload
+    ([lang|()],(p,p)) | p ∈ @Set.univ multi_payload
   }
-
-def cfg_expand : Set ( List (Symbol T N)) :=
-  {
-    c | cfg1.Generates c
-  }
-
-def lang_list_index : Set (List trm) :=
-  {l | (trm_to_symbol_list l) ∈ cfg_expand }
-
-def lang_index_only : Set trm :=
-  {squeeze_trm t | t ∈ lang_list_index}
-
 def lang_set : Set trm :=
   {l | cfg1.Generates (expand_trm l) ∧ l ∈ @Set.univ trm}
 
-def lang_index : Set (trm × payload ):=
-  { (l, (0)) | l ∈ lang_index_only}
+def lang_index : Set (trm × multi_payload × multi_payload ):=
+  { (l, ([0],[0])) | l ∈ lang_set}
 
 variable (pa_len : ℕ) (pb_len : ℕ) (xptr : loc)
-variable (paptr : trm × payload -> loc) (pbptr : trm × payload -> loc)
+variable (paptr : trm × multi_payload × multi_payload -> loc)
+ (pbptr : trm × multi_payload × multi_payload -> loc)
 
-lemma example4_spec' (f : ℤ -> val) (g q : ℤ -> val):
+lemma example4_spec' (f : ℤ -> val) (x : loc) (g q : ℤ -> val):
   {
     arr⟨⋆⟩(xptr , i in 1 =>f i)
+    -- check the syntax of x->_
+    -- ∗
+    -- bighstar ⟪0,pay_index⟫ (fun i => harray i.val.2.1 (paptr i.val) ∗ harray i.val.2.2 (pbptr i.val))
   }
-  [0| p in pay_index => prog_c1(⟨f 0⟩,⟨p.val.2⟩) ]
+  [0| p in pay_index => prog_c1(⟨f 0⟩,⸨pa:Loc⸩, ⸨pb:Loc⸩)]
   [1| l in lang_index => ⟦l.val.1⟧]
   { v,
     fun h => ∀ l ∈ lang_index, ∃ p ∈ pay_index , (fun ll pp => h ⟨1, ll⟩ = h ⟨0, pp⟩) l p
