WeirdLogic/WUtil.lean
@@ -1,0 +1,210 @@
+import WeirdLogic.Wlgtm
+
+open Lean Lean.Expr Lean.Meta Qq
+open Elab Command Term Meta Tactic
+open Classical trm val prim
+
+local macro "LabType" : term => `(ℕ)
+
+-- open prim val trm
+
+-- lemma arr_union_eq (f : ℤ -> val):
+--   s = s₁ ∪ s₂ ->
+--   Disjoint s₁ s₂ ->
+--   arr⟨s⟩(xptr , i in 1 =>f i) = arr⟨s₁⟩(xptr , i in 1 =>f i) ∗ arr⟨s₂⟩(xptr , i in 1 =>f i) := by
+--   move=> unio disj
+--   unfold hharrayFun
+--   rw [unio]
+--   apply eq_comm.mpr
+--   apply bighstar_hhstar_disj=>//
+
+#check heap
+#check bighstar_hhstar_disj
+#check bighstar_hhadd
+#check Set.diff_union_of_subset
+
+open EmptyPCM in
+lemma bighstar_hhstar_disj_dir
+   {hH : α -> hProp} {s₁ s₂ s: Set α} :
+    Disjoint s₁ s₂ ->
+    s = s₁ ∪ s₂ ->
+    [∗ i in s₁ | hH i] ∗ [∗ i in s₂ | hH i] = [∗ i in s | hH i] := by
+    move=>dj un ;rw [un]
+    srw -hhaddE; apply bighstar_hhadd_disj; exact dj
+
+lemma pair_set_union_right ( p₁ p₂ : Set α ) ( d : β ) :
+  p₁ ∩ p₂ = ∅ ->
+  {x | ∃ p ∈ p₁, (d, p) = x} ∩ {x | ∃ p ∈ p₂, (d, p) = x} = ∅ := by
+  move=> h
+  ext x
+  simp
+  intro p1 hp1 dph1 p2 hp2
+  subst dph1
+  simp_all only [Prod.mk.injEq, true_and]
+  intro heq
+  have hmem : p1 ∈ p₁ ∩ p₂ := ⟨hp1, heq ▸ hp2⟩
+  rw [h] at hmem
+  exact hmem
+
+lemma pair_set_union_index_right (i : ℕ) ( p₁ p₂ : Set α) ( d : β ) :
+  p₁ ∩ p₂ = ∅ ->
+  {x : (β × α)ˡ | ∃ p ∈ p₁, ⟨i, (d, p)⟩ = x} ∩ {x | ∃ p ∈ p₂, ⟨i,(d, p)⟩ = x} = ∅ := by
+  move=> h
+  ext x
+  simp
+  intro p1 hp1 dph1 p2 hp2
+  subst dph1
+  simp
+  intro heq
+  have hmem : p1 ∈ p₁ ∩ p₂ := ⟨hp1, heq ▸ hp2⟩
+  rw [h] at hmem
+  exact hmem
+
+lemma pair_set_union_left ( p₁ p₂ : Set α ) ( d : β ) :
+  p₁ ∩ p₂ = ∅ ->
+  {x | ∃ p ∈ p₁, (p, d) = x} ∩ {x | ∃ p ∈ p₂, (p, d) = x} = ∅ := by
+  move=> h
+  ext x
+  simp
+  intro p1 hp1 dph1 p2 hp2
+  subst dph1
+  simp_all only [Prod.mk.injEq, and_true]
+  intro heq
+  have hmem : p1 ∈ p₁ ∩ p₂ := ⟨hp1, heq ▸ hp2⟩
+  rw [h] at hmem
+  exact hmem
+
+lemma pair_set_union_index_left (i : ℕ) ( p₁ p₂ : Set α) ( d : β ) :
+  p₁ ∩ p₂ = ∅ ->
+  {x : (α × β)ˡ | ∃ p ∈ p₁, ⟨i, (p, d)⟩ = x} ∩ {x | ∃ p ∈ p₂, ⟨i,(p, d)⟩ = x} = ∅ := by
+  move=> h
+  ext x
+  simp
+  intro p1 hp1 dph1 p2 hp2
+  subst dph1
+  simp
+  intro heq
+  have hmem : p1 ∈ p₁ ∩ p₂ := ⟨hp1, heq ▸ hp2⟩
+  rw [h] at hmem
+  exact hmem
+
+lemma pair_set_union_eq_left ( p₁ p₂ p₃ : Set α ) ( d : β ) :
+  p₁ ∪ p₂ = p₃ ->
+  {x | ∃ p ∈ p₁, (d, p) = x} ∪ {x | ∃ p ∈ p₂, (d, p) = x} = {x | ∃ p ∈ p₃, (d, p) = x} := by
+  move=> h
+  aesop
+
+lemma pair_set_union_eq_right ( p₁ p₂ p₃ : Set α ) ( d : β ) :
+  p₁ ∪ p₂ = p₃ ->
+  {x | ∃ p ∈ p₁, (p, d) = x} ∪ {x | ∃ p ∈ p₂, (p, d) = x} = {x | ∃ p ∈ p₃, (p, d) = x} := by
+  move=> h
+  aesop
+
+lemma pair_set_union_index_eq_left ( p₁ p₂ p₃ : Set α ) ( d : β ) :
+  p₁ ∪ p₂ = p₃ ->
+  {x : (β × α)ˡ | ∃ p ∈ p₁, ⟨i, (d, p)⟩ = x} ∪ {x | ∃ p ∈ p₂, ⟨i, (d, p)⟩ = x} = {x | ∃ p ∈ p₃, ⟨i, (d, p)⟩ = x} := by
+  move=> h
+  aesop
+
+lemma pair_set_union_index_eq_right ( p₁ p₂ p₃ : Set α ) ( d : β ) :
+  p₁ ∪ p₂ = p₃ ->
+  {x : (α × β)ˡ | ∃ p ∈ p₁, ⟨i, (p, d)⟩ = x} ∪ {x | ∃ p ∈ p₂, ⟨i, (p, d)⟩ = x} = {x | ∃ p ∈ p₃, ⟨i, (p, d)⟩ = x} := by
+  move=> h
+  aesop
+
+lemma pair_insert_disjoin ( p₁ p₂ : Set α) ( a b : α) :
+  Disjoint p₁ p₂ ->
+  a ≠ b ->
+  a ∉ p₂ ->
+  b ∉ p₁ ->
+  insert a p₁ ∩ insert b p₂ = ∅ := by
+  move => dj ne na nb
+  ext x
+  simp [Set.ext_iff, Set.mem_insert_iff]
+  intro h
+  constructor
+  · aesop
+  · intro h2
+    by_cases h3 : x = a
+    · rw [h3] at h2
+      contradiction
+    · simp_all only [ne_eq, false_or]
+      have contra := Set.disjoint_iff.mp dj
+      simp_all only [Set.subset_empty_iff]
+      have hx : x ∈ p₁ ∩ p₂ := ⟨h, h2⟩
+      rw [contra] at hx
+      exact hx
+
+lemma psnd_eq ( d : β) ( s: Set (α × β)):
+  (∀ p ∈ s, p.snd = d) ->
+  ∀ b a, (a, b) ∈ s → d = b := by
+  intro hp b a hba
+  specialize hp (a, b) hba
+  simp_all
+
+lemma pair_wrap_eq_left {α β : Type} (i : ℕ) (d : β) (s' : Set α) (s : Set (α × β)) :
+  (∀ p ∈ s, p.snd = d) ->
+  (Prod.fst) '' s = s' ->
+  {x : (α × β)ˡ| ∃ p ∈ s, ⟨i, p⟩ = x} = {x | ∃ p ∈ s', ⟨i, (p, d)⟩ = x} := by
+  intro p hfst
+  ext x
+  simp [Set.mem_setOf_eq]
+  constructor
+  · simp
+    intro a b hba hiba
+    use a
+    constructor
+    · aesop
+    · have db_eq : d = b := psnd_eq d s p b a hba
+      rw [db_eq]
+      exact hiba
+  · simp
+    intro a hs hida
+    use a, d
+    constructor
+    · have ⟨b, hb⟩ : ∃ b, (a, b) ∈ s := by
+        rw [← hfst] at hs
+        aesop
+      have db_eq : d = b := psnd_eq d s p b a hb
+      rw [db_eq]
+      exact hb
+    · exact hida
+
+lemma pfst_eq ( d : β) ( s: Set (β × α)):
+  (∀ p ∈ s, p.fst = d) ->
+  ∀ b a, (b, a) ∈ s → d = b := by
+  intro hp b a hba
+  specialize hp (b, a) hba
+  simp_all
+
+lemma pair_wrap_eq_right {α β : Type} (i : ℕ) (d : β) (s' : Set α) (s : Set (β × α)) :
+  (∀ p ∈ s, p.fst = d )->
+  (Prod.snd) '' s = s' ->
+  {x : (β × α)ˡ| ∃ p ∈ s, ⟨i, p⟩ = x} = {x | ∃ p ∈ s', ⟨i, (d, p)⟩ = x} := by
+  intro p hsnd
+  ext x
+  simp [Set.mem_setOf_eq]
+  constructor
+  · simp
+    intro b a hba hiba
+    use a
+    constructor
+    · aesop
+    · have db_eq : d = b := pfst_eq d s p b a hba
+      rw [db_eq]
+      exact hiba
+  · simp
+    intro a hs hida
+    use d, a
+    constructor
+    · have ⟨b, hb⟩ : ∃ b, (b, a) ∈ s := by
+        rw [← hsnd] at hs
+        aesop
+      have db_eq : d = b := pfst_eq d s p b a hb
+      rw [db_eq]
+      exact hb
+    · exact hida
+
+lemma unsimp_singleton_set ( t : trm) ( p : β) :
+  {x | ∃ l ∈ ({t} : Set trm), (l, p) = x} = {(t, p)} := by
+  simp
